proofs/fstar/extraction-edited/Libcrux.Kem.Kyber.fst
@@ -10,7 +10,7 @@ let v_KEY_GENERATION_SEED_SIZE: usize =
   Libcrux.Kem.Kyber.Constants.v_CPA_PKE_KEY_GENERATION_SEED_SIZE +!
   Libcrux.Kem.Kyber.Constants.v_SHARED_SECRET_SIZE
 
-let decapsulate
+let decapsulate #p
       v_K v_SECRET_KEY_SIZE v_CPA_SECRET_KEY_SIZE v_PUBLIC_KEY_SIZE v_CIPHERTEXT_SIZE v_T_AS_NTT_ENCODED_SIZE v_C1_SIZE v_C2_SIZE v_VECTOR_U_COMPRESSION_FACTOR v_VECTOR_V_COMPRESSION_FACTOR v_C1_BLOCK_SIZE v_ETA1 v_ETA1_RANDOMNESS_SIZE v_ETA2 v_ETA2_RANDOMNESS_SIZE v_IMPLICIT_REJECTION_HASH_INPUT_SIZE
       (secret_key: Libcrux.Kem.Kyber.Types.t_KyberPrivateKey v_SECRET_KEY_SIZE)
       (ciphertext: Libcrux.Kem.Kyber.Types.t_KyberCiphertext v_CIPHERTEXT_SIZE) = 
@@ -24,9 +24,10 @@ let decapsulate
     Core.Slice.impl__split_at secret_key Libcrux.Kem.Kyber.Constants.v_H_DIGEST_SIZE
   in
   assert (length implicit_rejection_value = v_SECRET_KEY_SIZE -! v_CPA_SECRET_KEY_SIZE -! v_PUBLIC_KEY_SIZE -! Libcrux.Kem.Kyber.Constants.v_H_DIGEST_SIZE);
-  assert (length implicit_rejection_value <. v_IMPLICIT_REJECTION_HASH_INPUT_SIZE);
+  assert (length implicit_rejection_value = Spec.Kyber.v_SHARED_SECRET_SIZE);
+  assert (Spec.Kyber.v_SHARED_SECRET_SIZE <=. Spec.Kyber.v_IMPLICIT_REJECTION_HASH_INPUT_SIZE p);
   let decrypted:t_Array u8 (sz 32) =
-    Libcrux.Kem.Kyber.Ind_cpa.decrypt v_K
+    Libcrux.Kem.Kyber.Ind_cpa.decrypt #p v_K
       v_CIPHERTEXT_SIZE
       v_C1_SIZE
       v_VECTOR_U_COMPRESSION_FACTOR
@@ -54,6 +55,7 @@ let decapsulate
         <:
         t_Slice u8)
   in
+  Spec.Kyber.lemma_slice_append to_hash decrypted ind_cpa_public_key_hash Libcrux.Kem.Kyber.Constants.v_SHARED_SECRET_SIZE;
   let hashed:t_Array u8 (sz 64) =
     Libcrux.Kem.Kyber.Hash_functions.v_G (Rust_primitives.unsize to_hash <: t_Slice u8)
   in
@@ -87,7 +89,7 @@ let decapsulate
   in
   let expected_ciphertext, _:(Libcrux.Kem.Kyber.Types.t_KyberCiphertext v_CIPHERTEXT_SIZE &
     Core.Option.t_Option Libcrux.Kem.Kyber.Types.t_Error) =
-    Libcrux.Kem.Kyber.Ind_cpa.encrypt v_K v_CIPHERTEXT_SIZE v_T_AS_NTT_ENCODED_SIZE v_C1_SIZE
+    Libcrux.Kem.Kyber.Ind_cpa.encrypt #p v_K v_CIPHERTEXT_SIZE v_T_AS_NTT_ENCODED_SIZE v_C1_SIZE
       v_C2_SIZE v_VECTOR_U_COMPRESSION_FACTOR v_VECTOR_V_COMPRESSION_FACTOR v_C1_BLOCK_SIZE v_ETA1
       v_ETA1_RANDOMNESS_SIZE v_ETA2 v_ETA2_RANDOMNESS_SIZE ind_cpa_public_key decrypted
       pseudorandomness
@@ -101,10 +103,9 @@ let decapsulate
   Libcrux.Kem.Kyber.Constant_time_ops.select_shared_secret_in_constant_time shared_secret
     (Rust_primitives.unsize implicit_rejection_shared_secret <: t_Slice u8)
     selector in
-  admit(); // Panic Freedom Proved. Functional Correctness Assumed.
   res
 
-let encapsulate
+let encapsulate #p
       (v_K v_CIPHERTEXT_SIZE v_PUBLIC_KEY_SIZE v_T_AS_NTT_ENCODED_SIZE v_C1_SIZE v_C2_SIZE v_VECTOR_U_COMPRESSION_FACTOR v_VECTOR_V_COMPRESSION_FACTOR v_VECTOR_U_BLOCK_LEN v_ETA1 v_ETA1_RANDOMNESS_SIZE v_ETA2 v_ETA2_RANDOMNESS_SIZE:
           usize)
       (public_key: Libcrux.Kem.Kyber.Types.t_KyberPublicKey v_PUBLIC_KEY_SIZE)
@@ -139,6 +140,9 @@ let encapsulate
         <:
         t_Slice u8)
   in
+  assert (Seq.slice to_hash 0 (v Libcrux.Kem.Kyber.Constants.v_H_DIGEST_SIZE) == randomness);
+  Spec.Kyber.lemma_slice_append to_hash randomness (Spec.Kyber.v_H public_key.f_value) Libcrux.Kem.Kyber.Constants.v_H_DIGEST_SIZE;
+  assert (to_hash == Spec.Kyber.concat randomness (Spec.Kyber.v_H public_key.f_value));
   let hashed:t_Array u8 (sz 64) =
     Libcrux.Kem.Kyber.Hash_functions.v_G (Rust_primitives.unsize to_hash <: t_Slice u8)
   in
@@ -148,7 +152,7 @@ let encapsulate
   in
   let ciphertext, sampling_a_error:(Libcrux.Kem.Kyber.Types.t_KyberCiphertext v_CIPHERTEXT_SIZE &
     Core.Option.t_Option Libcrux.Kem.Kyber.Types.t_Error) =
-    Libcrux.Kem.Kyber.Ind_cpa.encrypt v_K v_CIPHERTEXT_SIZE v_T_AS_NTT_ENCODED_SIZE v_C1_SIZE
+    Libcrux.Kem.Kyber.Ind_cpa.encrypt #p v_K v_CIPHERTEXT_SIZE v_T_AS_NTT_ENCODED_SIZE v_C1_SIZE
       v_C2_SIZE v_VECTOR_U_COMPRESSION_FACTOR v_VECTOR_V_COMPRESSION_FACTOR v_VECTOR_U_BLOCK_LEN
       v_ETA1 v_ETA1_RANDOMNESS_SIZE v_ETA2 v_ETA2_RANDOMNESS_SIZE
       (Rust_primitives.unsize (Libcrux.Kem.Kyber.Types.impl_24__as_slice v_PUBLIC_KEY_SIZE
@@ -179,10 +183,9 @@ let encapsulate
       (Libcrux.Kem.Kyber.Types.t_KyberCiphertext v_CIPHERTEXT_SIZE & t_Array u8 (sz 32))
       Libcrux.Kem.Kyber.Types.t_Error
   in
-  admit();  // Panic Freedom Proved. Functional Correctness Assumed.
   res 
 
-let generate_keypair
+let generate_keypair #p
       (v_K v_CPA_PRIVATE_KEY_SIZE v_PRIVATE_KEY_SIZE v_PUBLIC_KEY_SIZE v_BYTES_PER_RING_ELEMENT v_ETA1 v_ETA1_RANDOMNESS_SIZE:
           usize)
       (randomness: t_Array u8 (sz 64)) = 
@@ -205,7 +208,7 @@ let generate_keypair
       v_CPA_PRIVATE_KEY_SIZE &
       Libcrux.Kem.Kyber.Types.t_KyberPublicKey v_PUBLIC_KEY_SIZE) &
     Core.Option.t_Option Libcrux.Kem.Kyber.Types.t_Error) =
-    Libcrux.Kem.Kyber.Ind_cpa.generate_keypair v_K
+    Libcrux.Kem.Kyber.Ind_cpa.generate_keypair #p v_K
       v_CPA_PRIVATE_KEY_SIZE
       v_PUBLIC_KEY_SIZE
       v_BYTES_PER_RING_ELEMENT
@@ -214,7 +217,7 @@ let generate_keypair
       ind_cpa_keypair_randomness
   in
   let secret_key_serialized:t_Array u8 v_PRIVATE_KEY_SIZE =
-    Libcrux.Kem.Kyber.Ind_cpa.serialize_secret_key v_PRIVATE_KEY_SIZE
+    Libcrux.Kem.Kyber.Ind_cpa.serialize_secret_key #p v_PRIVATE_KEY_SIZE
       (Rust_primitives.unsize (Libcrux.Kem.Kyber.Types.impl_30__as_slice v_CPA_PRIVATE_KEY_SIZE
               ind_cpa_private_key
             <:
@@ -231,13 +234,13 @@ let generate_keypair
   in
   let res = 
   match sampling_a_error with
-  | Core.Option.Option_Some error ->
+  | Core.Option.Option_Some error -> (
     Core.Result.Result_Err error
     <:
     Core.Result.t_Result
       (Libcrux.Kem.Kyber.Types.t_KyberKeyPair v_PRIVATE_KEY_SIZE v_PUBLIC_KEY_SIZE)
-      Libcrux.Kem.Kyber.Types.t_Error
-  | _ ->
+      Libcrux.Kem.Kyber.Types.t_Error)
+  | _ -> (
     let (private_key: Libcrux.Kem.Kyber.Types.t_KyberPrivateKey v_PRIVATE_KEY_SIZE):Libcrux.Kem.Kyber.Types.t_KyberPrivateKey
     v_PRIVATE_KEY_SIZE =
       Core.Convert.f_from secret_key_serialized
@@ -247,7 +250,6 @@ let generate_keypair
     <:
     Core.Result.t_Result
       (Libcrux.Kem.Kyber.Types.t_KyberKeyPair v_PRIVATE_KEY_SIZE v_PUBLIC_KEY_SIZE)
-      Libcrux.Kem.Kyber.Types.t_Error
+      Libcrux.Kem.Kyber.Types.t_Error)
   in 
-  admit();  // Panic Freedom Proved. Functional Correctness Assumed.
   res
