proofs/fstar/extraction-edited/Libcrux.Kem.Kyber.Kyber1024.fst
@@ -75,7 +75,7 @@ let decapsulate_1024_
       (secret_key: Libcrux.Kem.Kyber.Types.t_KyberPrivateKey (sz 3168))
       (ciphertext: Libcrux.Kem.Kyber.Types.t_KyberCiphertext (sz 1568))
     : t_Array u8 (sz 32) =
-  Libcrux.Kem.Kyber.decapsulate (sz 4) (sz 3168) (sz 1536) (sz 1568) (sz 1568) (sz 1536) (sz 1408)
+  Libcrux.Kem.Kyber.decapsulate #Spec.Kyber.kyber1024_params (sz 4) (sz 3168) (sz 1536) (sz 1568) (sz 1568) (sz 1536) (sz 1408)
     (sz 160) (sz 11) (sz 5) (sz 352) (sz 2) (sz 128) (sz 2) (sz 128) (sz 1600) secret_key ciphertext
 
 let encapsulate_1024_
@@ -84,7 +84,7 @@ let encapsulate_1024_
     : Core.Result.t_Result
       (Libcrux.Kem.Kyber.Types.t_KyberCiphertext (sz 1568) & t_Array u8 (sz 32))
       Libcrux.Kem.Kyber.Types.t_Error =
-  Libcrux.Kem.Kyber.encapsulate (sz 4) (sz 1568) (sz 1568) (sz 1536) (sz 1408) (sz 160) (sz 11)
+  Libcrux.Kem.Kyber.encapsulate #Spec.Kyber.kyber1024_params (sz 4) (sz 1568) (sz 1568) (sz 1536) (sz 1408) (sz 160) (sz 11)
     (sz 5) (sz 352) (sz 2) (sz 128) (sz 2) (sz 128) public_key randomness
 
 let generate_key_pair_1024_ (randomness: t_Array u8 (sz 64))
