proofs/fstar/extraction-edited/Libcrux.Kem.Kyber.Kyber512.fst
@@ -75,7 +75,7 @@ let decapsulate_512_
       (secret_key: Libcrux.Kem.Kyber.Types.t_KyberPrivateKey (sz 1632))
       (ciphertext: Libcrux.Kem.Kyber.Types.t_KyberCiphertext (sz 768))
     : t_Array u8 (sz 32) =
-  Libcrux.Kem.Kyber.decapsulate (sz 2) (sz 1632) (sz 768) (sz 800) (sz 768) (sz 768) (sz 640)
+  Libcrux.Kem.Kyber.decapsulate #Spec.Kyber.kyber512_params (sz 2) (sz 1632) (sz 768) (sz 800) (sz 768) (sz 768) (sz 640)
     (sz 128) (sz 10) (sz 4) (sz 320) (sz 3) (sz 192) (sz 2) (sz 128) (sz 800) secret_key ciphertext
 
 let encapsulate_512_
@@ -83,7 +83,7 @@ let encapsulate_512_
       (randomness: t_Array u8 (sz 32))
     : Core.Result.t_Result (Libcrux.Kem.Kyber.Types.t_KyberCiphertext (sz 768) & t_Array u8 (sz 32))
       Libcrux.Kem.Kyber.Types.t_Error =
-  Libcrux.Kem.Kyber.encapsulate (sz 2) (sz 768) (sz 800) (sz 768) (sz 640) (sz 128) (sz 10) (sz 4)
+  Libcrux.Kem.Kyber.encapsulate #Spec.Kyber.kyber512_params (sz 2) (sz 768) (sz 800) (sz 768) (sz 640) (sz 128) (sz 10) (sz 4)
     (sz 320) (sz 3) (sz 192) (sz 2) (sz 128) public_key randomness
 
 let generate_key_pair_512_ (randomness: t_Array u8 (sz 64))
