proofs/fstar/extraction-edited/Libcrux.Kem.Kyber.Kyber768.fst
@@ -65,14 +65,14 @@ let v_IMPLICIT_REJECTION_HASH_INPUT_SIZE: usize =
 let decapsulate_768_
       (secret_key: Libcrux.Kem.Kyber.Types.t_KyberPrivateKey (sz 2400))
       (ciphertext: Libcrux.Kem.Kyber.Types.t_KyberCiphertext (sz 1088)) =
-  Libcrux.Kem.Kyber.decapsulate (sz 3) (sz 2400) (sz 1152) (sz 1184) (sz 1088) (sz 1152) (sz 960)
+  Libcrux.Kem.Kyber.decapsulate #Spec.Kyber.kyber768_params (sz 3) (sz 2400) (sz 1152) (sz 1184) (sz 1088) (sz 1152) (sz 960)
     (sz 128) (sz 10) (sz 4) (sz 320) (sz 2) (sz 128) (sz 2) (sz 128) (sz 1120) secret_key ciphertext
 
 
 let encapsulate_768_
       (public_key: Libcrux.Kem.Kyber.Types.t_KyberPublicKey (sz 1184))
       (randomness: t_Array u8 (sz 32)) =
-  Libcrux.Kem.Kyber.encapsulate (sz 3) (sz 1088) (sz 1184) (sz 1152) (sz 960) (sz 128) (sz 10)
+  Libcrux.Kem.Kyber.encapsulate #Spec.Kyber.kyber768_params (sz 3) (sz 1088) (sz 1184) (sz 1152) (sz 960) (sz 128) (sz 10)
     (sz 4) (sz 320) (sz 2) (sz 128) (sz 2) (sz 128) public_key randomness
 
 let generate_key_pair_768_ (randomness: t_Array u8 (sz 64)) =
