proofs/fstar/extraction-edited/Libcrux.Kem.Kyber.fsti
@@ -3,26 +3,28 @@ module Libcrux.Kem.Kyber
 open Core
 open FStar.Mul
 
-val decapsulate
+val decapsulate (#p:Spec.Kyber.params)
       (v_K v_SECRET_KEY_SIZE v_CPA_SECRET_KEY_SIZE v_PUBLIC_KEY_SIZE v_CIPHERTEXT_SIZE v_T_AS_NTT_ENCODED_SIZE v_C1_SIZE v_C2_SIZE v_VECTOR_U_COMPRESSION_FACTOR v_VECTOR_V_COMPRESSION_FACTOR v_C1_BLOCK_SIZE v_ETA1 v_ETA1_RANDOMNESS_SIZE v_ETA2 v_ETA2_RANDOMNESS_SIZE v_IMPLICIT_REJECTION_HASH_INPUT_SIZE:
           usize)
       (secret_key: Libcrux.Kem.Kyber.Types.t_KyberPrivateKey v_SECRET_KEY_SIZE)
       (ciphertext: Libcrux.Kem.Kyber.Types.t_KyberCiphertext v_CIPHERTEXT_SIZE)
     : Pure (t_Array u8 (sz 32))
-    (requires (let p = let open Spec.Kyber in {v_RANK = v_K; v_ETA1; v_ETA2; v_VECTOR_U_COMPRESSION_FACTOR; v_VECTOR_V_COMPRESSION_FACTOR} in
+    (requires ( p == (let open Spec.Kyber in {v_RANK = v_K; v_ETA1; v_ETA2; v_VECTOR_U_COMPRESSION_FACTOR; v_VECTOR_V_COMPRESSION_FACTOR}) /\
                 Spec.Kyber.valid_params p /\
                 v_IMPLICIT_REJECTION_HASH_INPUT_SIZE == Spec.Kyber.v_IMPLICIT_REJECTION_HASH_INPUT_SIZE p /\
                 v_SECRET_KEY_SIZE == Spec.Kyber.v_SECRET_KEY_SIZE p /\
                 v_CPA_SECRET_KEY_SIZE == Spec.Kyber.v_CPA_PKE_SECRET_KEY_SIZE p /\
                 v_PUBLIC_KEY_SIZE == Spec.Kyber.v_CPA_PKE_PUBLIC_KEY_SIZE p /\
-                v_CIPHERTEXT_SIZE == Spec.Kyber.v_CPA_PKE_CIPHERTEXT_SIZE p
+                v_CIPHERTEXT_SIZE == Spec.Kyber.v_CPA_PKE_CIPHERTEXT_SIZE p /\
+                v_C1_SIZE == Spec.Kyber.v_C1_SIZE p /\
+                v_T_AS_NTT_ENCODED_SIZE = Spec.Kyber.v_T_AS_NTT_ENCODED_SIZE p
                ))
     (ensures (fun res ->
                 let open Spec.Kyber in
                 let p = {v_RANK = v_K; v_ETA1; v_ETA2; v_VECTOR_U_COMPRESSION_FACTOR; v_VECTOR_V_COMPRESSION_FACTOR} in
                 res == Spec.Kyber.ind_cca_decapsulate p secret_key.f_value ciphertext.f_value))
 
-val encapsulate
+val encapsulate (#p:Spec.Kyber.params)
       (v_K v_CIPHERTEXT_SIZE v_PUBLIC_KEY_SIZE v_T_AS_NTT_ENCODED_SIZE v_C1_SIZE v_C2_SIZE v_VECTOR_U_COMPRESSION_FACTOR v_VECTOR_V_COMPRESSION_FACTOR v_VECTOR_U_BLOCK_LEN v_ETA1 v_ETA1_RANDOMNESS_SIZE v_ETA2 v_ETA2_RANDOMNESS_SIZE:
           usize)
       (public_key: Libcrux.Kem.Kyber.Types.t_KyberPublicKey v_PUBLIC_KEY_SIZE)
@@ -31,10 +33,12 @@ val encapsulate
            (Libcrux.Kem.Kyber.Types.t_KyberCiphertext v_CIPHERTEXT_SIZE & t_Array u8 (sz 32))
             Libcrux.Kem.Kyber.Types.t_Error)
       (requires (
-                let p = let open Spec.Kyber in {v_RANK = v_K; v_ETA1; v_ETA2; v_VECTOR_U_COMPRESSION_FACTOR; v_VECTOR_V_COMPRESSION_FACTOR} in
+                p == (let open Spec.Kyber in {v_RANK = v_K; v_ETA1; v_ETA2; v_VECTOR_U_COMPRESSION_FACTOR; v_VECTOR_V_COMPRESSION_FACTOR}) /\
                 Spec.Kyber.valid_params p /\
                 v_PUBLIC_KEY_SIZE == Spec.Kyber.v_CPA_PKE_PUBLIC_KEY_SIZE p /\
-                v_CIPHERTEXT_SIZE == Spec.Kyber.v_CPA_PKE_CIPHERTEXT_SIZE p
+                v_CIPHERTEXT_SIZE == Spec.Kyber.v_CPA_PKE_CIPHERTEXT_SIZE p /\
+                v_C1_SIZE == Spec.Kyber.v_C1_SIZE p /\
+                v_T_AS_NTT_ENCODED_SIZE = Spec.Kyber.v_T_AS_NTT_ENCODED_SIZE p
                 ))
 
       (ensures (fun res ->
@@ -54,6 +58,7 @@ val generate_keypair (#p:Spec.Kyber.params)
            Libcrux.Kem.Kyber.Types.t_Error)
       (requires (v_K == p.v_RANK /\ v_ETA1 == p.v_ETA1 /\
                 v_PUBLIC_KEY_SIZE == Spec.Kyber.v_CPA_PKE_PUBLIC_KEY_SIZE p /\
+                v_CPA_PRIVATE_KEY_SIZE == Spec.Kyber.v_CPA_PKE_SECRET_KEY_SIZE p /\
                 v_PRIVATE_KEY_SIZE == Spec.Kyber.v_SECRET_KEY_SIZE p
                 ))
 
